aligning with tests, part 1 (up to 102, except 58, 69, 77, 84, 90, 92)

016-count_distinct_characters.dfy
@@ -1,9 +1,10 @@
+//TODO: General form should accept all characters
 function contains_char(s: string, c: char): bool
   decreases |s|
-  requires forall i :: 0 <= i < |s| ==> 'a' <= s[i] <= 'z' || 'A' <= s[i] <= 'Z'
-  requires 'a' <= c <= 'z'
+  requires forall i :: 0 <= i < |s| ==> 'a' <= s[i] <= 'z' || 'A' <= s[i] <= 'Z' || s[i] == ' '
+  requires ('a' <= c <= 'z') || (c == ' ')
 {
-  if |s| == 0 then false else s[0] == c || s[0] == upper_char(c) || contains_char(s[1..], c)
+  if |s| == 0 then false else s[0] == c || (c != ' ' && s[0] == upper_char(c)) || contains_char(s[1..], c)
 }
 // pure-end
 function upper_char(c: char) : (C: char)
@@ -13,10 +14,10 @@ function upper_char(c: char) : (C: char)
 // pure-end
 method count_distinct_characters(s: string) returns (count: int)
   // pre-conditions-start
-  requires forall i :: 0 <= i < |s| ==> 'a' <= s[i] <= 'z' || 'A' <= s[i] <= 'Z'
+  requires forall i :: 0 <= i < |s| ==> 'a' <= s[i] <= 'z' || 'A' <= s[i] <= 'Z' || s[i] == ' '
   // pre-conditions-end
   // post-conditions-start
-  ensures count == |set c | 'a' <= c <= 'z' && contains_char(s, c)|
+  ensures count == |set c | (('a' <= c <= 'z') || (c == ' ')) && contains_char(s, c)|
   // post-conditions-end
 {
   // impl-start
@@ -37,5 +38,10 @@ method count_distinct_characters(s: string) returns (count: int)
     i := (i as int + 1) as char;
   }
   assert contained == set c | 'a' <= c <= 'z' && contains_char(s, c); // assert-line
+  if contains_char(s, ' ') {
+    count := count + 1;
+    contained := contained + {' '};
+  }
+  assert contained == set c | (('a' <= c <= 'z') || (c == ' ')) && contains_char(s, c); // assert-line
   // impl-end
 }
