051-remove-vowels.dfy
@@ -1,8 +1,13 @@
+function is_vowel(c: char) : bool
+{
+    c == 'a' || c == 'e' || c == 'i' || c == 'o' || c == 'u' || c == 'A' || c == 'E' || c == 'I' || c == 'O' || c == 'U'
+}
+
 method remove_vowels(text : string) returns (s : string)
     // post-conditions-start
-    ensures forall i : int :: i >= 0 && i < |s| ==> s[i] != 'a' && s[i] != 'e' && s[i] != 'i' && s[i] != 'o' && s[i] != 'u'
+    ensures forall i : int :: i >= 0 && i < |s| ==> !is_vowel(s[i])
     ensures forall i : int :: i >= 0 && i < |s| ==> s[i] in text
-    ensures forall j : int :: j >= 0 && j < |text| && text[j] != 'a' && text[j] != 'e' && text[j] != 'i' && text[j] != 'o' && text[j] != 'u' ==> text[j] in s
+    ensures forall j : int :: j >= 0 && j < |text| && !is_vowel(text[j]) ==> text[j] in s
     // post-conditions-end
 {
     // impl-start
@@ -11,13 +16,13 @@ method remove_vowels(text : string) returns (s : string)
     while (i < |text|)
         // invariants-start
         invariant 0 <= i && i <= |text|
-        invariant forall i : int :: i >= 0 && i < |s| ==> s[i] != 'a' && s[i] != 'e' && s[i] != 'i' && s[i] != 'o' && s[i] != 'u'
+        invariant forall i : int :: i >= 0 && i < |s| ==> !is_vowel(s[i])
         invariant forall i : int :: i >= 0 && i < |s| ==> s[i] in text
-        invariant forall j : int :: j >= 0 && j < i && text[j] != 'a' && text[j] != 'e' && text[j] != 'i' && text[j] != 'o' && text[j] != 'u' ==> text[j] in s
+        invariant forall j : int :: j >= 0 && j < i && !is_vowel(text[j]) ==> text[j] in s
         // invariants-end
     {
         var c : char := text[i];
-        if (c != 'a' && c != 'e' && c != 'i' && c != 'o' && c != 'u')
+        if (!is_vowel(c))
         {
             s := s + [c];
         }
