066-digitSum.dfy
@@ -1,20 +1,20 @@
-function upper_sum_rec(s: string): int
+function digitSum_rec(s: string): int
   // post-conditions-start
-  ensures upper_sum_rec(s) >= 0
+  ensures digitSum_rec(s) >= 0
   // post-conditions-end
 {
   // impl-start
   if |s| == 0 then
     0
   else
-    var remaining := upper_sum_rec(s[1..]);
+    var remaining := digitSum_rec(s[1..]);
     to_int(s[0]) + remaining
   // impl-end
 }
 
-lemma upper_sum_rec_prop(s: string)
+lemma digitSum_rec_prop(s: string)
   requires |s| > 0
-  ensures upper_sum_rec(s) == upper_sum_rec(s[..|s|-1]) + to_int(s[|s|-1])
+  ensures digitSum_rec(s) == digitSum_rec(s[..|s|-1]) + to_int(s[|s|-1])
 {
     if (|s| > 1) {
         assert (s[1..][..|s[1..]| - 1]) == s[1..|s| - 1];
@@ -28,9 +28,9 @@ function to_int(c: char): int
     if 'A' <= c <= 'Z' then c as int else 0
 }
 // pure-end
-method upper_sum(s: string) returns (res: int)
+method digitSum(s: string) returns (res: int)
     // post-conditions-start
-    ensures res == upper_sum_rec(s)
+    ensures res == digitSum_rec(s)
     // post-conditions-end
 {
     // impl-start
@@ -39,14 +39,14 @@ method upper_sum(s: string) returns (res: int)
     while (i < |s|)
         // invariants-start
         invariant 0 <= i <= |s|
-        invariant res == upper_sum_rec(s[..i])
+        invariant res == digitSum_rec(s[..i])
         // invariants-end
     {
         res := res + to_int(s[i]);
         // assert-start
-        assert upper_sum_rec(s[..i + 1]) == upper_sum_rec(s[..i]) + to_int(s[i]) by {
+        assert digitSum_rec(s[..i + 1]) == digitSum_rec(s[..i]) + to_int(s[i]) by {
             assert s[..i+1][..i] == s[..i];
-            upper_sum_rec_prop(s[..i + 1]);
+            digitSum_rec_prop(s[..i + 1]);
         }
         // assert-end
         i := i + 1;
