031-is-prime.dfy
@@ -1,13 +1,17 @@
 method is_prime(k: int) returns (result: bool)
   // pre-conditions-start
-  requires k >= 2
+  requires k >= 1
   // pre-conditions-end
   // post-conditions-start
   ensures result ==> forall i :: 2 <= i < k ==> k % i != 0
-  ensures !result ==> exists j :: 2 <= j < k && k % j == 0
+  ensures (k > 1 && !result) ==> exists j :: 2 <= j < k && k % j == 0
   // post-conditions-end
 {
   // impl-start
+  if k == 1 {
+    result := false;
+    return;
+  }
   result := true;
   for i := 2 to k
     // invariants-start
