076-is_simple_power.dfy
@@ -12,38 +12,38 @@ lemma power_monotonic(x: nat, y: nat, j: nat)
     ensures power(x, j) >= power(x, y)
 {}
 // pure-end
-method is_simple_power(x: nat, n: int) returns (ans : bool)
+method is_simple_power(x: int, n: nat) returns (ans : bool)
     // pre-conditions-start
-    requires x > 0
+    requires n > 0
     // pre-conditions-end
     // post-conditions-start
-    ensures ans <==> exists y :: n == power(x, y)
+    ensures ans <==> exists y :: x == power(n, y)
     // post-conditions-end
 {
     // impl-start
-    if(x == 1) {
+    if(n == 1) {
         // assert-start
-        assert forall y :: power(x, y) == 1 by { forall y { power_unit(y); } }
+        assert forall y :: power(n, y) == 1 by { forall y { power_unit(y); } }
         // assert-end
-        assert n == 1 ==> n == power(x, 1); // assert-line
-        return n == 1;
+        assert x == 1 ==> x == power(n, 1); // assert-line
+        return x == 1;
     }
     var acc := 1;
     var i := 0;
-    while(acc < n)
+    while(acc < x)
         // invariants-start
-        invariant acc == power(x, i)
-        invariant forall j : nat :: j < i ==> power(x, j) < n
+        invariant acc == power(n, i)
+        invariant forall j : nat :: j < i ==> power(n, j) < x
         // invariants-end
     {
-        acc := x * acc;
+        acc := n * acc;
         i := i + 1;
     }
-    if(acc == n) {
+    if(acc == x) {
         return true;
     } else {
         // assert-start
-        assert forall j : nat :: j >= i ==> power(x, j) > n by { forall j | j > i { power_monotonic(x, i, j); } }
+        assert forall j : nat :: j >= i ==> power(n, j) > x by { forall j | j > i { power_monotonic(n, i, j); } }
         // assert-end
         return false;
     }
