090-next_smallest.dfy
@@ -9,7 +9,7 @@ function getVal(mx : Option<int>) : int
     }
 }
 // pure-end
-method rolling_max(s: seq<int>) returns (res: Option<int>) 
+method next_smallest(s: seq<int>) returns (res: Option<int>)
     // post-conditions-start
     ensures res == None <==> |s| < 2
     ensures res != None ==> exists x :: 0 <= x < |s| && s[x] == getVal(res)
